Ordered_Resolution_Prover/Abstract_Substitution.thy
@@ -154,6 +154,9 @@ locale substitution = substitution_ops subst_atm id_subst comp_subst
     subst_atm :: "'a \<Rightarrow> 's \<Rightarrow> 'a" and
     id_subst :: 's and
     comp_subst :: "'s \<Rightarrow> 's \<Rightarrow> 's" +
+  fixes 
+(* FIXME: Come up with a better name? Function gives substitutions that standardize clauses apart. Also rename it in the other locales. *)
+    mk_var_dis :: "'a literal multiset list \<Rightarrow> 's list"
   assumes
     subst_atm_id_subst[simp]: "subst_atm A id_subst = A" and
     subst_atm_comp_subst[simp]: "subst_atm A (comp_subst \<tau> \<sigma>) = subst_atm (subst_atm A \<tau>) \<sigma>" and
@@ -161,10 +164,14 @@ locale substitution = substitution_ops subst_atm id_subst comp_subst
     make_ground_subst:
       "is_ground_cls_list (CC \<cdot>cl \<sigma>) \<Longrightarrow>
        \<exists>\<tau>. is_ground_subst \<tau> \<and> (\<forall>i < length CC. \<forall>S. S \<subseteq># CC ! i \<longrightarrow> S \<cdot> \<sigma> = S \<cdot> \<tau>)" and
-    make_var_disjoint: "\<And>Cs. \<exists>\<rho>s. length \<rho>s = length Cs \<and> (\<forall>\<rho> \<in> set \<rho>s. is_renaming \<rho>) \<and>
-      var_disjoint (Cs \<cdot>\<cdot>cl \<rho>s)" and
+    mk_var_dis_p: "\<And>Cs. length (mk_var_dis Cs) = length Cs \<and> (\<forall>\<rho> \<in> set (mk_var_dis Cs). is_renaming \<rho>) \<and>
+       var_disjoint (Cs \<cdot>\<cdot>cl (mk_var_dis Cs))" and
     proper_instance_of_wf: "wfP proper_instance_of"
 begin
+
+lemma make_var_disjoint: "\<And>Cs. \<exists>\<rho>s. length \<rho>s = length Cs \<and> (\<forall>\<rho> \<in> set \<rho>s. is_renaming \<rho>) \<and>
+      var_disjoint (Cs \<cdot>\<cdot>cl \<rho>s)"
+  using mk_var_dis_p by auto
 
 lemma subst_ext_iff: "\<sigma> = \<tau> \<longleftrightarrow> (\<forall>A. A \<cdot>a \<sigma> = A \<cdot>a \<tau>)"
   by (blast intro: subst_ext)
@@ -907,11 +914,12 @@ end
 
 subsection \<open>Unification\<close>
 
-locale unification = substitution subst_atm id_subst comp_subst
+locale unification = substitution subst_atm id_subst comp_subst mk_var_dis
   for
     subst_atm :: "'a \<Rightarrow> 's \<Rightarrow> 'a" and
     id_subst :: 's and
-    comp_subst :: "'s \<Rightarrow> 's \<Rightarrow> 's" +
+    comp_subst :: "'s \<Rightarrow> 's \<Rightarrow> 's" and
+    mk_var_dis :: "'a literal multiset list \<Rightarrow> 's list" +
   fixes
     mgu :: "'a set set \<Rightarrow> 's option"
   assumes
